Generated/erc20shim/ERC20Shim/Common/if_5327145078839977110_gen.lean
@@ -1,6 +1,6 @@
 import Clear.ReasoningPrinciple
 
-import Generated.erc20shim.ERC20Shim.Common.if_3856757177752523473
+import Generated.erc20shim.ERC20Shim.Common.if_2130076443351184838
 import Generated.erc20shim.ERC20Shim.abi_encode_address_uint256_uint256
 import Generated.erc20shim.ERC20Shim.fun__approve
 
@@ -11,46 +11,46 @@ section
 
 open Clear EVMState Ast Expr Stmt FunctionDefinition State Interpreter ExecLemmas OutOfFuelLemmas Abstraction YulNotation PrimOps ReasoningPrinciple Utilities ERC20Shim.Common Generated.erc20shim ERC20Shim
 
-def if_8475192588736690919 := <s
-  if _2 
+def if_5327145078839977110 := <s
+  if _3 
 {
-    let _3 := lt(var_currentAllowance, var_value)
-    if _3 
+    let _4 := lt(var_currentAllowance, var_value)
+    if _4 
     {
         let expr := var_spender
         let expr_1 := var_currentAllowance
         let expr_2 := var_value
-        let _4 := 64
-        let _5 := mload(_4)
-        let _6 := shl(225, 2110234841)
-        mstore(_5, _6)
-        let _7 := 4
-        let _8 := add(_5, _7)
-        let _9 := abi_encode_address_uint256_uint256(_8, var_spender, var_currentAllowance, var_value)
-        let _10 := sub(_9, _5)
-        revert(_5, _10)
+        let _5 := 64
+        let _6 := mload(_5)
+        let _7 := shl(225, 2110234841)
+        mstore(_6, _7)
+        let _8 := 4
+        let _9 := add(_6, _8)
+        let _10 := abi_encode_address_uint256_uint256(_9, var_spender, var_currentAllowance, var_value)
+        let _11 := sub(_10, _6)
+        revert(_6, _11)
     }
     let expr_3 := var_owner
     let expr_4 := var_spender
-    let _11 := 0
-    let _12 := sub(var_currentAllowance, var_value)
-    fun__approve(var_owner, var_spender, _12, _11)
+    let _12 := 0
+    let _13 := sub(var_currentAllowance, var_value)
+    fun__approve(var_owner, var_spender, _13, _12)
 }
 >
 
 set_option maxRecDepth 5000
 set_option maxHeartbeats 400000
 
-def if_8475192588736690919_concrete_of_code : {
+def if_5327145078839977110_concrete_of_code : {
     C : State → State → Prop
     // ∀ {s₀ s₉ fuel}
-    , exec fuel if_8475192588736690919 s₀ = s₉
+    , exec fuel if_5327145078839977110 s₀ = s₉
     → Spec C s₀ s₉
   } := by
   constructor
   intros s₀ s₉ fuel
 
-  unfold Spec if_8475192588736690919
+  unfold Spec if_5327145078839977110
   rcases s₀ with ⟨evm₀, store₀⟩ | _ | c <;> dsimp only
   rotate_left 1
   · generalize If _ _ = f; aesop
@@ -74,7 +74,7 @@ def if_8475192588736690919_concrete_of_code : {
   -- abstraction offsetting
   rw [cons]
   generalize hxs : Block _ = xs
-  abstract if_3856757177752523473_abs_of_code if_3856757177752523473 with ss hs
+  abstract if_2130076443351184838_abs_of_code if_2130076443351184838 with ss hs
   try rw [← hs₁, hok] at hs
   intros h
   try intros h'
