Generated/erc20shim/ERC20Shim/fun_approve_426_gen.lean
@@ -9,8 +9,8 @@ section
 
 open Clear EVMState Ast Expr Stmt FunctionDefinition State Interpreter ExecLemmas OutOfFuelLemmas Abstraction YulNotation PrimOps ReasoningPrinciple Utilities Generated.erc20shim ERC20Shim
 
-def fun_approve_420 : FunctionDefinition := <f
-    function fun_approve_420(var_owner, var_spender, var_value) -> 
+def fun_approve_426 : FunctionDefinition := <f
+    function fun_approve_426(var_owner, var_spender, var_value) -> 
     
 {
     let expr := var_owner
@@ -23,18 +23,18 @@ def fun_approve_420 : FunctionDefinition := <f
 set_option maxRecDepth 4000
 set_option maxHeartbeats 300000
 
-def fun_approve_420_concrete_of_code
+def fun_approve_426_concrete_of_code
 : {
     C :
       _ → _ → _ → 
       State → State → Prop
     // ∀ {s₀ s₉ : State} { var_owner var_spender var_value fuel},
-         execCall fuel fun_approve_420 [] (s₀, [var_owner, var_spender, var_value]) = s₉ →
+         execCall fuel fun_approve_426 [] (s₀, [var_owner, var_spender, var_value]) = s₉ →
          Spec (C  var_owner var_spender var_value) s₀ s₉
   } := by
   constructor
   intros s₀ s₉  var_owner var_spender var_value fuel
-  unfold fun_approve_420
+  unfold fun_approve_426
 
   unfold Spec
   rcases s₀ with ⟨evm, store⟩ | _ | c <;> dsimp only
