Generated/erc20shim/ERC20Shim/fun_balanceOf.lean
@@ -13,9 +13,9 @@ section
 
 open Clear EVMState Ast Expr Stmt FunctionDefinition State Interpreter ExecLemmas OutOfFuelLemmas Abstraction YulNotation PrimOps ReasoningPrinciple Utilities Generated.erc20shim ERC20Shim
 
-lemma fun_balanceOf_abs_of_code {s₀ s₉ : State} {var var_account} {fuel : Nat} :
-  execCall fuel fun_balanceOf [var] (s₀, [var_account]) = s₉ →
-  Spec (A_fun_balanceOf var var_account) s₀ s₉
+lemma fun_balanceOf_abs_of_code {s₀ s₉ : State} {var_ var_account} {fuel : Nat} :
+  execCall fuel fun_balanceOf [var_] (s₀, [var_account]) = s₉ →
+  Spec (A_fun_balanceOf var_ var_account) s₀ s₉
 := λ h ↦ fun_balanceOf_abs_of_concrete (fun_balanceOf_concrete_of_code.2 h)
 
 end
